src/Std/Data/DTreeMap/Internal/WF/Lemmas.lean
@@ -592,9 +592,23 @@ theorem get!ₘ_eq_getValueCast! [Ord α] [TransOrd α] [LawfulEqOrd α] {k : α
     {t : Impl α β} (hto : t.Ordered) : t.get!ₘ k = getValueCast! k t.toListModel := by
   simp [get!ₘ, get?ₘ_eq_getValueCast? hto, getValueCast!_eq_getValueCast?]
 
-theorem get!_eq_getValueCast! [Ord α] [TransOrd α] [LawfulEqOrd α] {k : α} {t : Impl α β}
-    (hto : t.Ordered) : t.get! k = getValueCast! k t.toListModel := by
+theorem get!_eq_getValueCast! [Ord α] [TransOrd α] [LawfulEqOrd α] {k : α} [Inhabited (β k)]
+    {t : Impl α β} (hto : t.Ordered) : t.get! k = getValueCast! k t.toListModel := by
   rw [get!_eq_get!ₘ, get!ₘ_eq_getValueCast! hto]
+
+/-!
+''' `getD`
+-/
+
+theorem getDₘ_eq_getValueCastD [Ord α] [TransOrd α] [LawfulEqOrd α] {k : α}
+    {t : Impl α β} {fallback : β k} (hto : t.Ordered) :
+    t.getDₘ k fallback = getValueCastD k t.toListModel fallback := by
+  simp [getDₘ, get?ₘ_eq_getValueCast? hto, getValueCastD_eq_getValueCast?]
+
+theorem getD_eq_getValueCastD [Ord α] [TransOrd α] [LawfulEqOrd α] {k : α}
+    {t : Impl α β} {fallback : β k} (hto : t.Ordered) :
+    t.getD k fallback = getValueCastD k t.toListModel fallback := by
+  rw [getD_eq_getDₘ, getDₘ_eq_getValueCastD hto]
 
 namespace Const
 
@@ -618,6 +632,53 @@ theorem get?ₘ_eq_getValue? [Ord α] [TransOrd α] {k : α} {t : Impl α (fun _
 theorem get?_eq_getValue? [Ord α] [TransOrd α] {k : α} {t : Impl α (fun _ => β)} (hto : t.Ordered) :
     get? k t = getValue? k t.toListModel := by
   rw [get?_eq_get?ₘ, get?ₘ_eq_getValue? hto]
+
+/-!
+''' `get`
+-/
+
+theorem contains_eq_get?ₘ_isSome [Ord α] [TransOrd α] {k : α} {t : Impl α β}
+    (hto : t.Ordered) : contains k t = (get?ₘ k t).isSome := by
+  rw [get?ₘ_eq_getValue? hto, contains_eq_containsKey hto, containsKey_eq_isSome_getValue?]
+
+theorem getₘ_eq_getValue [Ord α] [TransOrd α] {k : α} {t : Impl α β} (h) {h'}
+    (hto : t.Ordered) : getₘ k t h' = getValue k t.toListModel h := by
+  simp only [getₘ]
+  revert h'
+  rw [get?ₘ_eq_getValue? hto]
+  simp [getValue?_eq_some_getValue ‹_›]
+
+theorem get_eq_getValue [Ord α] [TransOrd α] {k : α} {t : Impl α β} {h}
+    (hto : t.Ordered): get k t h = getValue k t.toListModel (contains_eq_containsKey hto ▸ h) := by
+  rw [get_eq_getₘ, getₘ_eq_getValue _ hto]
+  exact contains_eq_get?ₘ_isSome hto ▸ h
+
+/-!
+''' `get!`
+-/
+
+theorem get!ₘ_eq_getValue! [Ord α] [TransOrd α] {k : α} [Inhabited β]
+    {t : Impl α β} (hto : t.Ordered) : get!ₘ k t = getValue! k t.toListModel := by
+  simp [get!ₘ, get?ₘ_eq_getValue? hto, getValue!_eq_getValue?]
+
+theorem get!_eq_getValue! [Ord α] [TransOrd α] {k : α} [Inhabited β]
+    {t : Impl α β} (hto : t.Ordered) : get! k t = getValue! k t.toListModel := by
+  rw [get!_eq_get!ₘ, get!ₘ_eq_getValue! hto]
+
+/-!
+''' `getD`
+-/
+
+theorem getDₘ_eq_getValueD [Ord α] [TransOrd α] {k : α}
+    {t : Impl α β} {fallback : β} (hto : t.Ordered) :
+    getDₘ k t fallback = getValueD k t.toListModel fallback := by
+  simp [getDₘ, get?ₘ_eq_getValue? hto, getValueD_eq_getValue?]
+
+theorem getD_eq_getValueD [Ord α] [TransOrd α] {k : α}
+    {t : Impl α β} {fallback : β} (hto : t.Ordered) :
+    getD k t fallback = getValueD k t.toListModel fallback := by
+  rw [getD_eq_getDₘ, getDₘ_eq_getValueD hto]
+
 
 end Const
 
